ber_fetch_tag proof skeleton and loop invariant [skip ci]

src/Lib/BCT/BFT/Vst.v
@@ -1,45 +1,223 @@
 Require Import Core.Core Core.StructNormalizer VstLib.
 Require Import VST.floyd.proofauto.
-Require Import BFT.Exec.
+(* Require Import BFT.Exec. *)
 Require Import Clight.ber_tlv_tag.
+Require Import Core.Notations Core.SepLemmas Core.Tactics Core.VstTactics.
 
 Definition Vprog : varspecs. mk_varspecs prog. Defined.
 Instance CompSpecs : compspecs. make_compspecs prog. Defined.
-  
+ 
+Open Scope int.
+ 
+Fixpoint aux_loop (ptr : list int) val skip size tclass tag sizeofval := 
+  match ptr with
+  | oct :: xs => if skip <=? size
+                then if negb (oct & Int.repr 128 == 0)
+                     then let val' := (val << Int.repr 7) or (oct & Int.repr 127) in
+                          if negb (val >> Int.repr (8 * sizeofval - 9) == 0)
+                          then (Int.neg 1, tag)
+                          else aux_loop xs val' (skip + 1)%Z size tclass tag sizeofval
+                     else let val' := (val << Int.repr 7) or oct in
+                         (Int.repr skip, (val' << Int.repr 2) or tclass)
+               else (0, tag)
+  | nil => (0, tag)
+  end.
+
+Definition bft_loop (ptr : list int) val size tclass tag sizeofval
+  := aux_loop (skipn 1 ptr) val 2 size tclass tag sizeofval.
+
+
+Definition ber_fetch_tags (ptr : list int) size tag sizeofval  :=
+  if eq_dec size 0%Z
+  then (0, tag)
+  else let val := Znth 0 ptr in 
+       let tclass := val >> Int.repr 6 in 
+       if eq_dec (val & Int.repr 31) (Int.repr 31)
+       then bft_loop ptr 0 size tclass tag sizeofval    
+       else (1, ((val & Int.repr 31) << Int.repr 2) or tclass).
+
 Open Scope Z.
 
 Section Ber_fetch_tag.
 
 Definition ber_fetch_tag_spec : ident * funspec :=
   DECLARE _ber_fetch_tag
-    WITH ptr_b : block, ptr_ofs : ptrofs, ptr_v : list Z, size : Z, 
+    WITH b : block, i : ptrofs, 
+         data : list int, size : Z, 
          tag_p : val
     PRE [tptr tvoid, tuint, tptr tuint]
       PROP (0 <= size <= Int.max_unsigned;
-           (* Zlength ptr_v = size; *)
-            Forall (fun x => 0 <= x <= Byte.max_unsigned) ptr_v;
-            Ptrofs.unsigned ptr_ofs + (Zlength ptr_v) < Ptrofs.modulus
-           (* 0 <= tag_v <= Int.max_unsigned; *)
-           )
-      PARAMS ((Vptr ptr_b ptr_ofs); Vint (Int.repr size); tag_p)
+            Forall (fun x => 0 <= Int.unsigned x <= Byte.max_unsigned) data;
+            Ptrofs.unsigned i + (Zlength data) < Ptrofs.modulus;
+            0 < len data)
+      PARAMS ((Vptr b i); Vint (Int.repr size); tag_p)
       GLOBALS ()
-      SEP (data_at Tsh (tarray tuchar (Zlength ptr_v)) 
-                   (map Vint (map Int.repr ptr_v)) (Vptr ptr_b ptr_ofs);
+      SEP (data_at Tsh (tarray tuchar (Zlength data)) 
+                   (map Vint data) (Vptr b i);
            data_at_ Tsh tuint tag_p)
     POST [tint]
-      let r := ber_fetch_tags ptr_v size 0 (sizeof tuint) in
+      let r := ber_fetch_tags data size 0%int (sizeof tuint) in
       PROP ()
-      LOCAL (temp ret_temp (Vint (Int.repr (fst r))))
-      SEP (data_at Tsh (tarray tuchar (Zlength ptr_v)) 
-                   (map Vint (map Int.repr ptr_v)) (Vptr ptr_b ptr_ofs);
-           data_at Tsh tuint (Vubyte (Byte.repr (snd r))) tag_p).
+      LOCAL (temp ret_temp (Vint (fst r)))
+      SEP (data_at Tsh (tarray tuchar (Zlength data)) 
+                   (map Vint data) (Vptr b i);
+           if eq_dec (fst r) 1%int 
+           then data_at Tsh tuint (Vint ((snd r))) tag_p
+           else data_at_ Tsh tuint tag_p).
 
 Definition Gprog := ltac:(with_library prog [ber_fetch_tag_spec]).
+
+Lemma Znth_0_cons_sublist :  forall (ls : list int) i, 
+             0 <= i < len ls ->
+             Znth i ls :: sublist (i + 1) (len ls) ls = sublist i (len ls) ls.
+  { intros.
+    erewrite Znth_cons_sublist.
+    autorewrite with sublist.
+    auto. lia. }
+Qed.
 
 Theorem ber_fetch_tag : semax_body Vprog Gprog 
                                    (normalize_function f_ber_fetch_tag composites) 
                                    ber_fetch_tag_spec.
 Proof.
+  start_function.
+  forward_if.
+  forward.
+  assert (data_at Tsh (tarray tuchar (len data)) (map Vint data) (Vptr b i) =
+          (data_at Tsh tuchar (Vint (Znth 0 data)) (Vptr b i) *
+          data_at Tsh (tarray tuchar (len data - 1)) 
+                  (sublist 1 (len data) (map Vint data))
+                  (Vptr b (i + 1)%ptrofs))%logic) as D.
+  { erewrite split_non_empty_list 
+      with (i := Vint (Znth 0 data)) 
+           (j2 := len data - 1) 
+           (ls' := sublist 1 (len data) (map Vint data)).
+    auto. erewrite <- map_sublist;
+            erewrite <- map_cons;
+            f_equal; erewrite Znth_0_cons_sublist; try lia; auto.
+    all: autorewrite with sublist; strip_repr. }
+  erewrite D.
+  Intros.
+  forward.
+  entailer!.
+  eapply Forall_Znth with (i0 := 0) in H0; try lia.
+  repeat forward.
+  forward_if.
+  repeat forward.
+  erewrite <- D.
+  unfold ber_fetch_tags.
+  repeat rewrite_if_b.
+  entailer!.
+  repeat forward.
+  (* Loop *)
+  Open Scope int.
+  match goal with
+  | [ _ : _ |-  semax _ ?P ?C ?Post ] =>
+    forward_loop (
+               EX j : Z, EX v : int, 
+                 PROP ( )
+                 LOCAL (temp _skipped (Vint (Int.repr 2));
+                        temp _ptr (Vptr b (i + Ptrofs.repr j)%ptrofs);
+                        temp _val (Vint (Int.or (v << Int.repr 7)
+                                                 ((Znth j data) & Int.repr 127)));
+                        temp _t'1 (Vint (Znth 0 data & Int.repr 31)%int);
+                        temp _tclass (Vint (Znth 0 data >> Int.repr 6)%int);
+                        temp _size (Vint (Int.repr size));
+                        temp _tag_r tag_p)
+                 SEP (data_at Tsh tuchar (Vint (Znth 0 data)) (Vptr b i);
+                      data_at Tsh (tarray tuchar (len data - 1)) 
+                              (sublist 1 (len data) (map Vint data))
+                              (Vptr b (i + 1)%ptrofs);
+                      data_at_ Tsh tuint tag_p))
+            break:
+             (EX j : Z, EX v : int,
+               let val := (Int.or (v << Int.repr 7) (Znth j data)) in
+               PROP (v >> Int.repr (8 * (sizeof tuint) - 9) <> 0) 
+                LOCAL (temp _skipped (Vint (Int.repr 2));
+                        temp _ptr (Vptr b (i + Ptrofs.repr j)%ptrofs);
+                        temp _val (Vint val);
+                        temp _t'1 (Vint (Znth 0 data & Int.repr 31)%int);
+                        temp _tclass (Vint (Znth 0 data >> Int.repr 6)%int);
+                        temp _size (Vint (Int.repr size));
+                        temp _tag_r tag_p)
+                 SEP (data_at Tsh tuchar (Vint (Znth 0 data)) (Vptr b i);
+                      data_at Tsh (tarray tuchar (len data - 1)) 
+                              (sublist 1 (len data) (map Vint data))
+                              (Vptr b (i + 1)%ptrofs);
+                      data_at Tsh tuint
+                              (Vint ((val << Int.repr 2) or
+                                 (Znth 0 data >> Int.repr 6)%int)) tag_p))
+  end.
+  -- (* PRE to LI *) 
+    Exists 1%Z 0.
+    entailer!.
+    admit.
+  -- (* LI C LI *)
+    forward_if.
+    ++ 
+      assert (data_at Tsh (tarray tuchar (len data - 1)) 
+                  (sublist 1 (len data) (map Vint data))
+                  (Vptr b (i + 1)%ptrofs) =
+          (data_at Tsh tuchar (Vint (Znth 1 data)) (Vptr b (i + 1)%ptrofs) *
+          data_at Tsh (tarray tuchar (len data - 2)) 
+                  (sublist 2 (len data) (map Vint data))
+                  (Vptr b (i + 1 + 1)%ptrofs))%logic) as D2.
+  { erewrite split_non_empty_list 
+      with (i := Vint (Znth 1 data)) 
+           (j2 := len data - 2) 
+           (ls' := sublist 2 (len data) (map Vint data)).
+    auto.  repeat erewrite <- map_sublist.
+    erewrite <- map_cons.
+    f_equal. erewrite Znth_0_cons_sublist; try lia; auto.
+    admit. (* 0 <= 1 < len data *)
+    all: autorewrite with sublist; strip_repr.
+    admit. admit.
+  }
+   erewrite D2.
+  Intros.
+  forward.
+  entailer!.
+  eapply Forall_Znth with (i0 := 1) in H0; try lia.
+  admit. (* 0 <= 1 < len data *)
+  forward_if.
+      ** forward.
+         forward_if.
+         forward.
+         entailer!.
+         (* -1 case *)
+         admit.
+         rewrite if_false by admit.
+         erewrite sepcon_comm.
+         erewrite sepcon_assoc.
+         erewrite <- D2.
+         erewrite <- D.
+         entailer!.
+         repeat forward.
+         entailer!.
+         admit.
+         erewrite <- D2.
+         entailer!.
+      ** repeat forward.
+         entailer!.
+         (* return skipped case *)
+         admit.
+         rewrite if_false by admit.
+         erewrite sepcon_comm.
+         erewrite sepcon_assoc.
+         erewrite <- D2.
+         erewrite <- D.
+         entailer!.
+    ++ forward.
+       entailer!.
+  --  (* BREAK rest POST *)
+    forward.
+    entailer!.
+    (* return 0 *)
+    admit.
+    rewrite if_false by admit.
+    erewrite sepcon_comm.
+    erewrite <- D.
+    entailer!.
 Admitted.
 
 End Ber_fetch_tag.
